Mbse/TextbookExercises/Registry.lean
@@ -72,7 +72,7 @@ def registry : List ExerciseEntry :=
   , ⟨"4.85", 4, .theoremProof, "solved", "Ch04.ex4_85_rearrangement_isomorphic"⟩
   , ⟨"4.86", 4, .theoremProof, "solved", "Ch04.ex4_86_nested_coupling_isomorphic"⟩
   , ⟨"5.141", 5, .theoremProof, "counterexample", "Ch05.subsystem_isSystemMode_or_counterexample"⟩
-  , ⟨"5.142", 5, .theoremProof, "qualified", "Ch05.exercise5_142_unconditional"⟩
+  , ⟨"5.142", 5, .theoremProof, "counterexample", "Ch05.systemMode_not_subsystem_counterexample"⟩
   , ⟨"5.146", 5, .theoremProof, "solved", "Ch05.selfMode_constantTime_iterate"⟩
   , ⟨"5.147", 5, .theoremProof, "solved", "Ch05.constantMode_state_at_mul"⟩
   , ⟨"5.148", 5, .theoremProof, "solved", "Ch05.variableTime_constantInput_state_at_accumulatedTime"⟩
